@prefix dcterms: <http://purl.org/dc/terms/> .
@prefix dt: <http://resource.geosciml.org/datatype/> .
@prefix rdf: <http://www.w3.org/1999/02/22-rdf-syntax-ns#> .
@prefix rdfs: <http://www.w3.org/2000/01/rdf-schema#> .
@prefix sdo: <https://schema.org/> .
@prefix skos: <http://www.w3.org/2004/02/skos/core#> .
@prefix xml: <http://www.w3.org/XML/1998/namespace> .
@prefix xsd: <http://www.w3.org/2001/XMLSchema#> .

<https://geo-carto.github.io/vocabularios/geomorfologia-actividad> a skos:ConceptScheme ;
    dcterms:created "2025-07-29"^^xsd:date ;
    dcterms:modified "2025-07-29"^^xsd:date ;
    dcterms:provenance "Términos originales de INSPIRE" ;
    dcterms:publisher "https://www.igme.es/" ; 
    dcterms:source "nan" ;
    skos:changeNote "2025-07-29. Generate SKOS encoding of vocabulary from Excel spreadsheet"@es ;
    skos:editorialNote "Este archivo contiene el vocabulario https://geo-carto.github.io/vocabularios/geomorfologia-actividad."@es ;
    skos:hasTopConcept <https://geo-carto.github.io/vocabularios/geomorfologia-actividad/activo>,
        <https://geo-carto.github.io/vocabularios/geomorfologia-actividad/latente>,
        <https://geo-carto.github.io/vocabularios/geomorfologia-actividad/reactivado>,
        <https://geo-carto.github.io/vocabularios/geomorfologia-actividad/estabilizado>,
    <https://geo-carto.github.io/vocabularios/geomorfologia-actividad/inactivo> ;
    skos:prefLabel "Actividad geomorfológica"@es ;
    skos:prefLabel "Geomorphologic activity"@en .


<https://geo-carto.github.io/vocabularios/geomorfologia-actividad/collection> a skos:Collection ;
    dcterms:provenance "este vocabulario" ;
    skos:definition "Todos los conceptos en este vocabulario." ;
    skos:member <https://geo-carto.github.io/vocabularios/geomorfologia-actividad/activo> ,
        <https://geo-carto.github.io/vocabularios/geomorfologia-actividad/latente> ,
        <https://geo-carto.github.io/vocabularios/geomorfologia-actividad/reactivado> ,
        <https://geo-carto.github.io/vocabularios/geomorfologia-actividad/estabilizado> ,
    <https://geo-carto.github.io/vocabularios/geomorfologia-actividad/inactivo> ;
    skos:prefLabel "https://geo-carto.github.io/vocabularios/geomorfologia-actividad - Todos los conceptos"@es .


<https://geo-carto.github.io/vocabularios/geomorfologia-actividad/activo> a skos:Concept ;
    dcterms:provenance "this vocabulary"@en ;
    rdfs:isDefinedBy <https://geo-carto.github.io/vocabularios/geomorfologia-actividad> ;
    skos:definition "A geomorphologic process that is currently in a state of action, or that has been reactivated since a conventionally short period of time."@es ,
         "A geomorphologic process that is currently in a state of action, or that has been reactivated since a conventionally short period of time."@en ;
    skos:inScheme <https://geo-carto.github.io/vocabularios/geomorfologia-actividad> ;
    skos:prefLabel "activo"@es ,
        "active"@en .

<https://geo-carto.github.io/vocabularios/geomorfologia-actividad/latente> a skos:Concept ;
    dcterms:provenance "this vocabulary"@en ;
    rdfs:isDefinedBy <https://geo-carto.github.io/vocabularios/geomorfologia-actividad> ;
    skos:definition "A geomorphologic process that has not shown signs of activity since a conventionally short period of time, and that could be reactivated by its original causes, or triggered by induced causes such as anthropogenic activities."@es ,
         "A geomorphologic process that has not shown signs of activity since a conventionally short period of time, and that could be reactivated by its original causes, or triggered by induced causes such as anthropogenic activities."@en ;
    skos:inScheme <https://geo-carto.github.io/vocabularios/geomorfologia-actividad> ;
    skos:prefLabel "latente"@es ,
        "dormant"@en .

<https://geo-carto.github.io/vocabularios/geomorfologia-actividad/reactivado> a skos:Concept ;
    dcterms:provenance "this vocabulary"@en ;
    rdfs:isDefinedBy <https://geo-carto.github.io/vocabularios/geomorfologia-actividad> ;
    skos:definition "A reactivated geomorphologic process is an active geomorphologic process which has been dormant."@es ,
         "A reactivated geomorphologic process is an active geomorphologic process which has been dormant."@en ;
    skos:inScheme <https://geo-carto.github.io/vocabularios/geomorfologia-actividad> ;
    skos:prefLabel "reactivado"@es ,
        "reactivated"@en .

<https://geo-carto.github.io/vocabularios/geomorfologia-actividad/estabilizado> a skos:Concept ;
    dcterms:provenance "this vocabulary"@en ;
    rdfs:isDefinedBy <https://geo-carto.github.io/vocabularios/geomorfologia-actividad> ;
    skos:definition "A stabilized geomorphologic process is an inactive process which has been protected from its original causes by remedial measures."@es ,
         "A stabilized geomorphologic process is an inactive process which has been protected from its original causes by remedial measures."@en ;
    skos:inScheme <https://geo-carto.github.io/vocabularios/geomorfologia-actividad> ;
    skos:prefLabel "estabilizado"@es ,
        "stabilised"@en .

<https://geo-carto.github.io/vocabularios/geomorfologia-actividad/inactivo> a skos:Concept ;
    dcterms:provenance "this vocabulary"@en ;
    rdfs:isDefinedBy <https://geo-carto.github.io/vocabularios/geomorfologia-actividad> ;
    skos:definition "A relict or fossil geomorphologic process."@es ,
         "A relict or fossil geomorphologic process."@en ;
    skos:inScheme <https://geo-carto.github.io/vocabularios/geomorfologia-actividad> ;
    skos:prefLabel "inactivo"@es ,
        "inactive"@en .
